sketch linear scan register allocator, not sure if correct

bedrock2/src/RegAlloc.v
@@ -4,26 +4,32 @@ Require Import compiler.StateCalculus.
 Require Import compiler.NameGen.
 Require Import compiler.NameWithEq.
 Require Import riscv.util.BitWidths.
+Require Import Coq.Lists.List.
 
 Section RegAlloc.
 
   Context {Bw: BitWidths}.
 
-  Context {Name: NameWithEq}.
-  Notation var := (@name Name).
-  Notation func := (@name Name) (only parsing). (* TODO use separate names *)
+  Context {VarName: NameWithEq}.
+  Context {RegisterName: NameWithEq}.
+  Context {FuncName: NameWithEq}.
+  
+  Notation var := (@name VarName).
+  Notation register := (@name RegisterName).
+  Notation func := (@name FuncName).
 
   Existing Instance eq_name_dec.
 
-  Context {state: Type}.
-  Context {stateMap: Map state var (word wXLEN)}.
   Context {vars: Type}.
   Context {varset: set vars var}.
-  Context {NGstate: Type}.
-  Context {NG: NameGen var vars NGstate}.
 
-  Ltac state_calc := state_calc_generic (@name Name) (word wXLEN).
-  Ltac set_solver := set_solver_generic (@name Name).
+  Context {registers: Type}.
+  Context {registerset: set registers register}.
+
+  Context {alloc: Type}.
+  Context {allocMap: Map alloc var register}.
+
+  Local Notation stmt := (@stmt Bw VarName FuncName).
 
   (* set of variables which is certainly written while executing s *)
   Fixpoint certainly_written(s: stmt): vars :=
@@ -37,7 +43,7 @@ Section RegAlloc.
     | SLoop s1 cond s2 => certainly_written s1
     | SSeq s1 s2 => union (certainly_written s1) (certainly_written s2)
     | SSkip => empty_set
-    | SCall argnames fname resnames => empty_set (* TODO *)
+    | SCall argnames fname resnames => of_list resnames
     end.
 
   (* set of variables which is live before executing s *)
@@ -52,7 +58,210 @@ Section RegAlloc.
     | SLoop s1 cond s2 => union (live s1) (diff (live s2) (certainly_written s1))
     | SSeq s1 s2       => union (live s1) (diff (live s2) (certainly_written s1))
     | SSkip => empty_set
-    | SCall argnames fname resnames => empty_set (* TODO *)
+    | SCall argnames fname resnames => of_list argnames
+    end.
+
+  Definition TODO{T: Type}: T. Admitted.
+  
+  Definition restrict(s: alloc)(newDomain: vars): alloc := TODO.
+
+  (* TODO implement, and treat the case where no more registers are available *)
+  Definition pick(rs: registers): (register * registers) := TODO.
+
+  Definition domain: alloc -> vars := TODO.
+  Definition range: alloc -> registers := TODO.
+
+  Definition start_interval(current: vars * registers * alloc)(x: var)
+    : vars * registers * alloc :=
+    let '(o, a, m) := current in
+    let o := union o (singleton_set x) in
+    let '(r, a) := pick a in
+    let m := put m x r in
+    (o, a, m).
+
+  Fixpoint regalloc
+           (o: vars)             (* occupants: variables which currently occupy a register *)
+           (a: registers)        (* available registers (those not used currently) *)
+           (m: alloc)            (* mapping from variables to registers *)
+           (s: stmt)             (* current sub-statement *)
+           (l: vars)             (* variables which have a life after statement s *)
+    : (vars * registers * alloc) (* new occupants, new available registers, new mapping *)
+    :=
+    let o_original := o in
+    (* these are the variables which actually deserve to occupy a register: *)
+    let o := union (live s) (diff l (certainly_written s)) in
+    (* intervals which ended... *)
+    let dead := diff o_original o in
+    (* ... allow allow us to add new available registers to a: *)
+    let a := union a (range (restrict m dead)) in
+    match s with
+    | SLoad x _ | SLit x _ | SOp x _ _ _ | SSet x _ =>
+        match get m x with
+        | Some rx => (o, a, m) (* nothing to do because no new interval starts *)
+        | None    => start_interval (o, a, m) x
+        end
+    | SStore x y => (o, a, m)
+    | SIf cond s1 s2   =>
+        let '(o1, a1, m1) := regalloc o a  m  s1 l in
+        let '(o2, a2, m2) := regalloc o a1 m1 s2 l in
+        (union o1 o2, a2, m2)
+    | SLoop s1 cond s2 =>
+        let '(o, a, m) := regalloc o a m s1 (union (union (singleton_set cond) (live s2)) l) in
+        regalloc o a m s2 l
+    | SSeq s1 s2 =>
+        let '(o, a, m) := regalloc o a m s1 (union (live s2) l) in
+        regalloc o a m s2 l
+    | SSkip => (o, a, m)
+    | SCall argnames fname resnames => fold_left start_interval resnames (o, a, m) 
+    end.
+
+  Inductive inspect{T: Type}: T -> Prop := .
+
+  Goal forall o a m l cond s1 s2 s3, inspect (regalloc o a m (SSeq (SIf cond s1 s2) s3) l).
+    intros.
+    let b := eval cbv delta [regalloc] in regalloc in change regalloc with b.
+    cbv beta iota. fold regalloc.
+    simpl live.
+  Abort.
+
+  Variable dummy_register: register.
+
+  Definition make_total(m: alloc): var -> register :=
+    fun x => match get m x with
+          | Some r => r
+          | None => dummy_register
+          end.
+
+  Definition apply_alloc(m: var -> register): stmt -> @FlatImp.stmt Bw RegisterName FuncName :=
+    fix rec(s: stmt) :=
+      match s with
+      | SLoad x y => SLoad (m x) (m y)
+      | SStore x y => SStore (m x) (m y)
+      | SLit x v => SLit (m x) v
+      | SOp x op y z => SOp (m x) op (m y) (m z)
+      | SSet x y => SSet (m x) (m y)
+      | SIf cond s1 s2   => SIf (m cond) (rec s1) (rec s2)
+      | SLoop s1 cond s2 => SLoop (rec s1) (m cond) (rec s2)
+      | SSeq s1 s2 => SSeq (rec s1) (rec s2)
+      | SSkip => SSkip
+      | SCall argnames fname resnames => SCall (map m argnames) fname (map m resnames)
+      end.
+
+  Variable available_registers: registers. (* r1..r31 on RISCV *)
+
+  Definition register_allocation(s: stmt): @FlatImp.stmt Bw RegisterName FuncName :=
+    let '(_, _, m) := regalloc empty_set available_registers empty s empty_set in
+    apply_alloc (make_total m) s.
+
+  (******* below: failed versions: **********)
+
+  (* This is too verbose: *)
+  Fixpoint regalloc'''
+           (occupants: vars)       (* variables which currently occupy a register *)
+           (available: registers)  (* registers not used currently *)
+           (assignment: alloc)     (* mapping from variables to registers *)
+           (s: stmt)               (* current sub-statement 
+                                      Note: After s, more statements will be executed! *)
+           (afterlive: vars)       (* variables which have a life after statement s *)
+    : (vars * registers * alloc)   (* new occupants, new available registers, new assignment *)
+    :=
+    (* let's see if we can add any available registers: *)
+    let deadvars := diff occupants (union (live s) afterlive) in
+    let registers_of_deadvars := range (restrict assignment deadvars) in
+    (* What if a live variable x and a dead variable y are mapped to the same register r?
+       Then if y is in deadvars, x is not in "occupants", because any two vars mapped to the
+       same register cannot be in "occupants" at the same time.
+       So adding r to the available registers is safe because it is not needed by x nor by y
+       any more. *)
+    let available := union available registers_of_deadvars in
+    let occupants := live s in
+    let nop := (occupants, available, assignment) in
+    match s with
+    | SLoad x _ | SLit x _ | SOp x _ _ _ | SSet x _ =>
+        match get assignment x with
+        | Some rx => nop (* nothing to do because no new interval starts *)
+        | None => (* new interval starts *)
+            let occupants := union occupants (singleton_set x) in
+            let '(r, available) := pick available in
+            let assignment := put assignment x r in
+            (occupants, available, assignment)
+        end
+    | SStore x y => nop
+    | SIf cond s1 s2   => TODO (*
+        let '(occupants1, available1, assignment1) :=
+          regalloc''' occupants available  assignment  s1 in
+        let '(occupants2, available2, assignment2) := 
+          regalloc''' occupants available1 assignment1 s1 in
+        (union occupants1 occupants2, available2, assignment2) *)
+    | SLoop s1 cond s2 => TODO
+    | SSeq s1 s2 =>
+        let '(occupants, available, assignment) :=
+          regalloc''' occupants available assignment s1 (union (live s2) afterlive) in
+        regalloc''' occupants available assignment s2 afterlive
+    | SSkip => nop
+    | SCall argnames fname resnames => TODO
+    end.
+  
+  Fixpoint regalloc''(active: vars)(available: registers)(assignment: alloc)(s: stmt):
+    (vars * registers * alloc) :=
+    (* let's see if we can add any available registers: *)
+    let deadvars := diff active (live s) in (* <-- this should be a bigger set (really all) *)
+    let registers_of_deadvars := range (restrict assignment deadvars) in
+    (* What if a live variable x and a dead variable y are mapped to the same register r?
+       Then if y is in deadvars, x is not in "active", because any two vars mapped to the
+       same register cannot be in "active" at the same time.
+       So adding r to the available registers is safe because it is not needed by x nor by y
+       any more. *)
+    let available := union available registers_of_deadvars in
+    let active := live s in
+    let nop := (active, available, assignment) in
+    match s with
+    | SLoad x _ | SLit x _ | SOp x _ _ _ | SSet x _ =>
+        match get assignment x with
+        | Some rx => nop (* nothing to do because no new interval starts *)
+        | None => (* new interval starts *)
+            let active := union active (singleton_set x) in
+            let '(r, available) := pick available in
+            let assignment := put assignment x r in
+            (active, available, assignment)
+        end
+    | SStore x y => nop
+    | SIf cond s1 s2   =>
+        let '(active1, available1, assignment1) := regalloc'' active available  assignment  s1 in
+        let '(active2, available2, assignment2) := regalloc'' active available1 assignment1 s1 in
+        (union active1 active2, available2, assignment2)
+    | SLoop s1 cond s2 => TODO
+    | SSeq s1 s2       =>
+        let '(active, available, assignment) := regalloc'' active available assignment s1 in
+        regalloc'' active available assignment s2
+    | SSkip => nop
+    | SCall argnames fname resnames => TODO
+    end.
+
+  Fixpoint regalloc'(available: registers)(assignment: alloc)(s: stmt): (registers * alloc) :=
+    (* let's see if we can add any available registers: *)
+    let deadvars := diff (domain assignment) (live s) in
+    let registers_of_deadvars := range (restrict assignment deadvars) in
+    (* What if a live variable x and a dead variable y are mapped to the same register r?
+       Then y is in deadvars, so r will be added to the available registers, even though
+       it is still needed to hold the value of x -> bad *)
+    let available := union available registers_of_deadvars in
+    match s with
+    | SLoad x _ | SLit x _ | SOp x _ _ _ | SSet x _ =>
+        match get assignment x with
+        | Some rx => (* nothing to do because no new interval starts *)
+            (available, assignment)
+        | None => (* new interval starts *)
+            let '(r, available) := pick available in
+            let assignment := put assignment x r in
+            (available, assignment)
+        end
+    | SStore x y   => TODO
+    | SIf cond s1 s2   => TODO
+    | SLoop s1 cond s2 => TODO
+    | SSeq s1 s2       => TODO
+    | SSkip => (available, assignment)
+    | SCall argnames fname resnames => TODO
     end.
 
 End RegAlloc.
